@@ -1,76 +1,424 @@
+{-# LANGUAGE InstanceSigs #-}
 module SCE.Source where
 
+import qualified SCE.Core as C
+import qualified Test.QuickCheck as QC
+
 -- Note: Context is a Type and Environment is an Expression
-type Ctx      = Typ 
+type Ctx      = Typ
 type Env      = Exp
 type Name     = String
 type Result a = Either String a
 
+-- Expression types
 data Typ
   = Int
   | Unit
   | TyAnd Typ Typ
-  | TyArr Typ Typ
+  | TyArr Typ Typ      -- A -> B  (regular functions)
   | TyRcd Name Typ
-  | TyStruct SigTyp
+  | TyMod ModTyp        -- module type (first-class)
   deriving (Eq, Show)
 
-data SigTyp
-  = TySig  Typ SigTyp
-  | TyIntf [TyDecl]
+-- Module types (stratified)
+data ModTyp
+  = TyIntf Typ          -- sig ... end  (struct's type is just a Typ/interface)
+  | TyArrM Typ ModTyp   -- A ->m I  (functor: takes value, produces module)
   deriving (Eq, Show)
 
-data TyDecl
-  = TyVal   Name Typ
-  | TyMod   Name SigTyp
-  | TyFunct Name SigTyp SigTyp
-  deriving (Eq, Show)
- 
 data Exp
-  = Query
-  | Proj Exp Int
-  | Lit  Int
-  | UnitE
-  | Lam Typ Exp
-  | Box Exp Exp
-  | Clos Exp Typ Exp
-  | App Exp Exp
-  | Mrg Exp Exp
-  | Rec Name Exp
-  | RProj Exp Name
-  -- To be elaborated
-  | Mod Module
+  = Query                        -- ?  (reify environment)
+  | Proj Exp Int                 -- e.n  (de Bruijn projection)
+  | Lit  Int                     -- i
+  | UnitE                        -- unit
+  | Lam Typ Exp                  -- lam A. e
+  | Box Exp Exp                  -- e1 |> e2
+  | Clos Exp Typ Exp             -- <v, lam A. e>
+  | App Exp Exp                  -- e1 e2
+  | DMrg Exp Exp                 -- e1 #d e2  (dependent merge)
+  | Rec Name Exp                 -- {l = e}
+  | RProj Exp Name               -- e.l
+  -- Modules (not stratified, live in Exp)
+  | MStruct  Sandbox Exp     -- struct[s] A. e
+  | MFunctor Sandbox Typ Exp     -- functor[s] (A) e
+  | MClos Exp Typ Exp            -- module closure <env, A, body>
+  | MLink Exp Exp                -- Link(e1, e2)
+  -- More elaborated terms
+  | NMrg Exp Exp                 -- e1 #n e2  (non-dependent merge)
+  | Let Exp Typ Exp              -- let e1 : A in e2
+  | Open Exp Exp                 -- open e1 in e2
   deriving (Eq, Show)
 
--- To be elaborated
-data Module
-  = MVar     Name            -- M ~~> ?.M
-  | MStruct  [Decl]          -- struct decl1; ...; declN end
-  | MFunctor Name Typ Module -- functor (x : A) m end
-  | MLink    Module Module   -- Link(M1, M2)
+data Sandbox = Sandboxed | Open_
   deriving (Eq, Show)
 
-data Sandbox = Sandboxed | Open
-  deriving (Eq, Show)
+isValue :: Exp -> Bool
+isValue (Lit _)        = True
+isValue UnitE          = True
+isValue (Clos v _ _)   = isValue v
+isValue (MClos v _ _)  = isValue v
+isValue (DMrg v1 v2)   = isValue v1 && isValue v2
+isValue (NMrg v1 v2)   = isValue v1 && isValue v2
+isValue (Rec _ v)      = isValue v
+isValue _              = False
 
-data Decl
-  = DLet   Sandbox Name (Maybe Typ) Exp
-  | DMod   Sandbox Name (Maybe SigTyp) Module
-  | DFunct Sandbox Name SigTyp (Maybe SigTyp) Module
-  deriving (Eq, Show)
+lookupIdx :: Typ -> Int -> Result Typ
+lookupIdx (TyAnd _ b) 0 = pure b
+lookupIdx (TyAnd a _) n = lookupIdx a (n - 1)
+lookupIdx _ _            = Left "index out of bounds in context"
 
--- lookupv for runtime values (de Bruijn)
-lookupV :: Env -> Int -> Result Exp
-lookupV (Mrg _ v2) 0 = pure v2
-lookupV (Mrg v1 _) n = lookupV v1 (n - 1)
-lookupV _ _          = Left "lookupV: index out of bounds"
+containment :: Name -> Typ -> Result Typ
+containment l (TyRcd l' a)
+  | l == l'   = pure a
+  | otherwise = Left $ "label " ++ l ++ " not found"
+containment l (TyAnd b c) =
+  case (containment l b, containment l c) of
+    (Right a, Left _)  -> pure a
+    (Left _,  Right a) -> pure a
+    (Right _, Right _) -> Left $ "ambiguous label " ++ l
+    (Left _,  Left _)  -> Left $ "label " ++ l ++ " not found"
+containment l _ = Left $ "label " ++ l ++ " not found"
+
+elaborateTyp :: Typ -> C.Typ
+elaborateTyp Int          = C.Int
+elaborateTyp Unit         = C.Unit
+elaborateTyp (TyArr a b)  = C.TyArr (elaborateTyp a) (elaborateTyp b)
+elaborateTyp (TyAnd a b)  = C.TyAnd (elaborateTyp a) (elaborateTyp b)
+elaborateTyp (TyRcd l a)  = C.TyRcd l (elaborateTyp a)
+elaborateTyp (TyMod mt)   = elaborateModTyp mt
+
+elaborateModTyp :: ModTyp -> C.Typ
+elaborateModTyp (TyIntf a)    = elaborateTyp a
+elaborateModTyp (TyArrM a mt) = C.TyArr (elaborateTyp a) (elaborateModTyp mt)
+
+elaborate :: Ctx -> Exp -> Result (Typ, C.Exp)
+elaborate g e = case e of
+  Query -> pure (g, C.Query)
+  Lit n -> pure (Int, C.Lit n)
+  UnitE -> pure (Unit, C.UnitE)
+  Proj se n -> do
+    (b, ce) <- elaborate g se
+    a <- lookupIdx b n
+    pure (a, C.Proj ce n)
+  Lam tyA se -> do
+    (tyB, ce) <- elaborate (TyAnd g tyA) se
+    pure (TyArr tyA tyB, C.Lam (elaborateTyp tyA) ce)
+  Box se1 se2 -> do
+    (g', ce1) <- elaborate g se1
+    (a, ce2)  <- elaborate g' se2
+    pure (a, C.Box ce1 ce2)
+  Clos se1 tyA se2 -> do
+    (g', ce1)  <- elaborate g se1
+    (tyB, ce2) <- elaborate (TyAnd g' tyA) se2
+    pure (TyArr tyA tyB, C.Clos ce1 (elaborateTyp tyA) ce2)
+  App se1 se2 -> do
+    (ty1, ce1) <- elaborate g se1
+    (ty2, ce2) <- elaborate g se2
+    case ty1 of
+      TyArr tyA tyB
+        | tyA == ty2 -> pure (tyB, C.App ce1 ce2)
+        | otherwise  -> Left "App: argument type mismatch"
+      _ -> Left "App: not a function type"
+  DMrg se1 se2 -> do
+    (a, ce1) <- elaborate g se1
+    (b, ce2) <- elaborate (TyAnd g a) se2
+    pure (TyAnd a b, C.Mrg ce1 ce2)
+  NMrg se1 se2 -> do
+    (a, ce1) <- elaborate g se1
+    (b, ce2) <- elaborate g se2
+    let gT   = elaborateTyp g
+        body = C.Mrg
+                 (C.Box (C.Proj C.Query 0) ce1)
+                 (C.Box (C.Proj C.Query 1) ce2)
+        core = C.App (C.Lam gT body) C.Query
+    pure (TyAnd a b, core)
+  Rec l se -> do
+    (a, ce) <- elaborate g se
+    pure (TyRcd l a, C.Rec l ce)
+  RProj se l -> do
+    (b, ce) <- elaborate g se
+    a <- containment l b
+    pure (a, C.RProj ce l)
+  Let se1 tyA se2 -> do
+    (a, ce1) <- elaborate g se1
+    if a /= tyA
+      then Left "Let: annotation mismatch"
+      else do
+        (b, ce2) <- elaborate (TyAnd g tyA) se2
+        pure (b, C.App (C.Lam (elaborateTyp tyA) ce2) ce1)
+  Open se1 se2 -> do
+    (ty1, ce1) <- elaborate g se1
+    case ty1 of
+      TyRcd l a -> do
+        (b, ce2) <- elaborate (TyAnd g a) se2
+        pure (b, C.App (C.Lam (elaborateTyp a) ce2) (C.RProj ce1 l))
+      _ -> Left "Open: expected record type"
+  -- infstruct-sandboxed: Unit & A |- e : B ~> ce
+  --   ==> G |- struct[sandboxed] A. e : Sig(A, B) ~> box unit (lam [A] ce)
+  -- infstruct-open: G & A |- e : B ~> ce
+  --   ==> G |- struct[open] A. e : Sig(A, B) ~> box ctx (lam [A] ce)
+  MStruct sb se -> do
+    let ctx' = case sb of
+                 Sandboxed -> Unit
+                 Open_     -> g
+    (tyB, ce) <- elaborate ctx' se
+    let envCore = case sb of
+                    Sandboxed -> C.UnitE
+                    Open_     -> C.Query
+    pure (TyMod (TyIntf tyB), C.Box envCore ce)
+  -- inffunctor-sandboxed: Unit & A |- e : B ~> ce
+  --   ==> G |- functor[sandboxed](A) e : A -> B ~> box unit (lam [A] ce)
+  -- inffunctor-open: G & A |- e : B ~> ce
+  --   ==> G |- functor[open](A) e : A -> B ~> lam [A] ce
+  MFunctor sb tyA se -> do
+    let ctx' = case sb of
+                 Sandboxed -> TyAnd Unit tyA
+                 Open_     -> TyAnd g tyA
+    (tyB, ce) <- elaborate ctx' se
+    let mt = case tyB of
+               TyMod innerMt -> TyArrM tyA innerMt
+               _             -> TyArrM tyA (TyIntf tyB)
+    case sb of
+      Sandboxed ->
+        pure (TyMod mt, C.Box C.UnitE (C.Lam (elaborateTyp tyA) ce))
+      Open_ ->
+        pure (TyMod mt, C.Lam (elaborateTyp tyA) ce)
+  -- Module closure typing (runtime construct, like Clos)
+  MClos se1 tyA se2 -> do
+    (g', ce1)  <- elaborate g se1
+    (tyB, ce2) <- elaborate (TyAnd g' tyA) se2
+    let mt = case tyB of
+               TyMod innerMt -> TyArrM tyA innerMt
+               _             -> TyArrM tyA (TyIntf tyB)
+    pure (TyMod mt, C.Clos ce1 (elaborateTyp tyA) ce2)
+
+  -- infmodapp / linking: G |- e1 : Sig(A,B) ~> ce1, G |- e2 : A ~> ce2
+  --                      ==> G |- Link(e1, e2) : B ~> app ce1 ce2
+  MLink se1 se2 -> do
+    (ty1, ce1) <- elaborate g se1
+    (ty2, ce2) <- elaborate g se2
+    case ty1 of
+      TyMod (TyArrM tyA mt)
+        | tyA == ty2 -> pure (TyMod mt, C.App ce1 ce2)
+        | otherwise  -> Left $ "MLink: argument type mismatch, expected "
+                             ++ show tyA ++ " got " ++ show ty2
+      _ -> Left $ "MLink: not a functor type, got " ++ show ty1
+
+lookupV :: Exp -> Int -> Result Exp
+lookupV (DMrg _ v2) 0 = pure v2
+lookupV (DMrg v1 _) n = lookupV v1 (n - 1)
+lookupV (NMrg _ v2) 0 = pure v2
+lookupV (NMrg v1 _) n = lookupV v1 (n - 1)
+lookupV _ _            = Left "lookupV: index out of bounds"
+
+sel :: Exp -> Name -> Result Exp
+sel (Rec l v) l'
+  | l == l'   = pure v
+  | otherwise = Left $ "sel: label " ++ l' ++ " not found"
+sel (DMrg v1 v2) l = selMrg v1 v2 l
+sel (NMrg v1 v2) l = selMrg v1 v2 l
+sel _ l = Left $ "sel: label " ++ l ++ " not found"
+
+selMrg :: Exp -> Exp -> Name -> Result Exp
+selMrg v1 v2 l =
+  case (sel v1 l, sel v2 l) of
+    (Right v, Left _)  -> pure v
+    (Left _,  Right v) -> pure v
+    (Right _, Right _) -> Left $ "sel: ambiguous label " ++ l
+    (Left _,  Left _)  -> Left $ "sel: label " ++ l ++ " not found"
 
 bigStep :: Env -> Exp -> Result Exp
-bigStep env Query       = pure env
-bigStep env (Proj e' i) = do
-  v <- bigStep env e'
-  lookupV v i
-bigStep _ (Lit i)       = pure $ Lit i
-bigStep _ UnitE         = pure $ UnitE
-bigStep env (Lam ty e)  = pure $ Clos env ty e
-bigStep _ _ = Left "TODO: Implement"    
+bigStep env e = case e of
+  Query         -> pure env
+  Lit i         -> pure $ Lit i
+  UnitE         -> pure UnitE
+
+  Clos v ty body  | isValue v -> pure $ Clos v ty body
+  MClos v ty body | isValue v -> pure $ MClos v ty body
+
+  Proj e' n -> do
+    v <- bigStep env e'
+    lookupV v n
+
+  Lam ty body -> pure $ Clos env ty body
+
+  Box e1 e2 -> do
+    v1 <- bigStep env e1
+    bigStep v1 e2
+
+  App e1 e2 -> do
+    clos <- bigStep env e1
+    v2   <- bigStep env e2
+    case clos of
+      Clos v1 _ body  -> bigStep (DMrg v1 v2) body
+      MClos v1 _ body -> bigStep (DMrg v1 v2) body
+      _ -> Left "app: not a closure"
+
+  DMrg e1 e2 -> do
+    v1 <- bigStep env e1
+    v2 <- bigStep (DMrg env v1) e2
+    pure $ DMrg v1 v2
+
+  NMrg e1 e2 -> do
+    v1 <- bigStep env e1
+    v2 <- bigStep env e2
+    pure $ NMrg v1 v2
+
+  Rec l e1 -> do
+    v1 <- bigStep env e1
+    pure $ Rec l v1
+
+  RProj e1 l -> do
+    v1 <- bigStep env e1
+    sel v1 l
+
+  Let e1 _ e2 -> do
+    v1 <- bigStep env e1
+    bigStep (DMrg env v1) e2
+
+  Open e1 e2 -> do
+    v1 <- bigStep env e1
+    case v1 of
+      Rec _ v -> bigStep (DMrg env v) e2
+      _       -> Left "open: expected record value"
+
+  MStruct Sandboxed body -> bigStep UnitE body
+  MStruct Open_     body -> bigStep env body
+
+  MFunctor Sandboxed ty body -> pure $ MClos UnitE ty body
+  MFunctor Open_     ty body -> pure $ MClos env ty body
+
+  MLink e1 e2 -> do
+    mclos <- bigStep env e1
+    v2    <- bigStep env e2
+    case mclos of
+      MClos v1 _ body -> bigStep (DMrg v1 v2) body
+      Clos  v1 _ body -> bigStep (DMrg v1 v2) body
+      _ -> Left "link: not a module closure"
+
+  _ -> Left $ "bigStep: stuck on " ++ show e
+
+infer :: Ctx -> Exp -> Result Typ
+infer g e = fst <$> elaborate g e
+
+isRight :: Either a b -> Bool
+isRight (Right _) = True
+isRight _         = False
+
+-- Theorem: Type-Preserving Elaboration
+-- If G |-S e : A ~> ce, then [G] |-C ce : [A]
+prop_typePreservingElaboration :: Ctx -> Exp -> Bool
+prop_typePreservingElaboration g se =
+  case elaborate g se of
+    Right (a, ce) ->
+      C.infer (elaborateTyp g) ce == Right (elaborateTyp a)
+    Left _ -> True
+
+-- Theorem: Uniqueness of Type Inference
+prop_uniqueInference :: Ctx -> Exp -> Bool
+prop_uniqueInference g se =
+  case (elaborate g se, elaborate g se) of
+    (Right (a1, _), Right (a2, _)) -> a1 == a2
+    _ -> True
+
+-- Theorem: Uniqueness of Elaboration
+prop_uniqueElaboration :: Ctx -> Exp -> Bool
+prop_uniqueElaboration g se =
+  case (elaborate g se, elaborate g se) of
+    (Right (_, ce1), Right (_, ce2)) -> ce1 == ce2
+    _ -> True
+
+-- Theorem: Semantics Preservation
+-- Source big-step and core big-step agree on elaborated terms
+prop_semanticsPreservation :: Exp -> Bool
+prop_semanticsPreservation se =
+  case elaborate Unit se of
+    Right (_, ce) ->
+      case (bigStep UnitE se, C.bigStep C.UnitE ce) of
+        (Right sv, Right cv) ->
+          case (infer Unit sv, C.infer C.Unit cv) of
+            (Right sty, Right cty) -> elaborateTyp sty == cty
+            _ -> True
+        (Left _, Left _) -> True
+        _ -> False
+    Left _ -> True
+
+-- Theorem: Capability Safety / Sandbox Isolation
+-- Sandboxed modules produce the same value under any environment
+prop_sandboxIsolation :: Exp -> Exp -> Exp -> Bool
+prop_sandboxIsolation env1 env2 body =
+  not (isValue env1 && isValue env2) || (let sb = MStruct Sandboxed body
+                                         in case (bigStep env1 sb, bigStep env2 sb) of
+                                              (Right v1, Right v2) -> v1 == v2
+                                              (Left _, Left _)     -> True
+                                              _                    -> False)
+
+-- Theorem: Sandbox Functor Isolation
+prop_sandboxFunctorIsolation :: Exp -> Exp -> Typ -> Exp -> Bool
+prop_sandboxFunctorIsolation env1 env2 tyA body =
+  not (isValue env1 && isValue env2) || (let sb = MFunctor Sandboxed tyA body
+                                         in case (bigStep env1 sb, bigStep env2 sb) of
+                                              (Right v1, Right v2) -> v1 == v2
+                                              (Left _, Left _)     -> True
+                                              _                    -> False)
+
+-- Theorem: Separate Compilation
+-- Elaborating Link(M1, M2) = App([M1], [M2])
+prop_separateCompilation :: Exp -> Exp -> Bool
+prop_separateCompilation se1 se2 =
+  case elaborate Unit (MLink se1 se2) of
+    Right (_, cLinked) ->
+      case (elaborate Unit se1, elaborate Unit se2) of
+        (Right (_, ce1), Right (_, ce2)) ->
+          cLinked == C.App ce1 ce2
+        _ -> True
+    Left _ -> True
+
+-- Theorem: Secure Linking
+-- Sandboxed functor's body result is independent of link partner's value
+-- (when body doesn't use the argument)
+prop_secureLinking :: Exp -> Exp -> Bool
+prop_secureLinking arg1 arg2 =
+  not (isValue arg1 && isValue arg2) || (let m = MFunctor Sandboxed Int (Lit 42)  -- doesn't use arg
+                                         in case (bigStep UnitE (MLink m arg1), bigStep UnitE (MLink m arg2)) of
+                                              (Right v1, Right v2) -> v1 == v2
+                                              (Left _, Left _)     -> True
+                                              _                    -> False)
+
+-- Theorem: Link Elaboration Commutes with Evaluation
+-- eval([Link(M1,M2)]) = eval(App([M1], [M2]))
+prop_linkElaborationCommutes :: Exp -> Exp -> Bool
+prop_linkElaborationCommutes se1 se2 =
+  case (elaborate Unit (MLink se1 se2), elaborate Unit se1, elaborate Unit se2) of
+    (Right (_, cLinked), Right (_, ce1), Right (_, ce2)) ->
+      case (C.bigStep C.UnitE cLinked, C.bigStep C.UnitE (C.App ce1 ce2)) of
+        (Right v1, Right v2) -> v1 == v2
+        (Left _, Left _)     -> True
+        _                    -> False
+    _ -> True
+
+-- Theorem: NMrg Independence
+-- In non-dependent merge, e2's type is independent of e1
+prop_nmrgIndependence :: Exp -> Exp -> Bool
+prop_nmrgIndependence se1 se2 =
+  case elaborate Unit (NMrg se1 se2) of
+    Right (TyAnd _ b, _) ->
+      case elaborate Unit se2 of
+        Right (b', _) -> b == b'
+        Left _        -> True
+    _ -> True
+
+-- Sanity: DMrg allows dependency (e2 can see e1's binding)
+prop_dmrgAllowsDependency :: Bool
+prop_dmrgAllowsDependency =
+  case elaborate Unit (DMrg (Lit 1) (Proj Query 0)) of
+    Right (TyAnd Int Int, _) -> True
+    _                        -> False
+
+-- Sanity: Struct elaborates to box env (lam A ce) in core
+prop_structShape :: Exp -> Bool
+prop_structShape body =
+  case elaborate Unit (MStruct Sandboxed body) of
+    Right (_, C.Box C.UnitE _) -> True
+    Right _  -> False
+    Left _   -> True
